[Dafny] Factor out dafny_remove_assert into its own file

compiler/dafny/proofs/dafny_compilerProofScript.sml
@@ -3,8 +3,9 @@
 *)
 Theory dafny_compilerProof
 Ancestors
-  dafny_semanticPrimitives dafny_freshen dafny_freshenProof
-  dafny_evaluateProps
+  dafny_semanticPrimitives dafny_evaluateProps
+  dafny_freshen dafny_freshenProof
+  dafny_remove_assert dafny_remove_assertProof
   dafny_to_cakeml dafny_to_cakemlProof dafny_compiler
   mlstring (* isPrefix *)
   primTypes evaluate semanticPrimitives namespace
@@ -24,6 +25,8 @@ Proof
   Cases_on ‘l’ \\ gvs []
 QED
 
+(* has_main is preserved throughout the compiler passes *)
+
 Theorem has_main_freshen[local]:
   has_main (freshen_program prog) =
   has_main prog
@@ -42,10 +45,20 @@ Proof
   \\ gvs [ZIP_EQ_NIL, UNZIP_EQ_NIL]
 QED
 
-Definition valid_members_def:
-  valid_members (Program members) =
-  EVERY (λmember. ALL_DISTINCT (get_param_names member)) members
-End
+Theorem has_main_remove_assert[local]:
+  has_main (remove_assert prog) = has_main prog
+Proof
+  namedCases_on ‘prog’ ["members"]
+  \\ simp [remove_assert_def]
+  \\ Induct_on ‘members’
+  >- (simp [remove_assert_member_def])
+  \\ qx_gen_tac ‘member’
+  \\ gvs [has_main_def, get_member_def, get_member_aux_def]
+  \\ Cases_on ‘member’ \\ simp [remove_assert_member_def]
+  \\ IF_CASES_TAC \\ gvs []
+QED
+
+(* -- *)
 
 Definition cml_init_state_def:
   cml_init_state ffi ck =
@@ -91,353 +104,8 @@ Proof
   gvs [cml_init_state_def]
 QED
 
-(* -- TODO Move to appropriate place -- *)
-open dafny_evaluateTheory;
-open dafny_astTheory;
-
-Definition remove_assert_stmt_def:
-  remove_assert_stmt (Assert _) = Skip ∧
-  remove_assert_stmt (Then stmt₁ stmt₂) =
-    Then (remove_assert_stmt stmt₁) (remove_assert_stmt stmt₂) ∧
-  remove_assert_stmt (If cnd thn els) =
-    If cnd (remove_assert_stmt thn) (remove_assert_stmt els) ∧
-  remove_assert_stmt (Dec lcl stmt) =
-    Dec lcl (remove_assert_stmt stmt) ∧
-  remove_assert_stmt (While grd invs decrs mod body) =
-    While grd invs decrs mod (remove_assert_stmt body) ∧
-  remove_assert_stmt stmt = stmt
-End
-
-Definition remove_assert_member_def:
-  remove_assert_member (Method name ins req ens reads decreases outs mod body) =
-    Method name ins req ens reads decreases outs mod (remove_assert_stmt body) ∧
-  remove_assert_member member = member
-End
-
-Definition remove_assert_def:
-  remove_assert (Program members) =
-    Program (MAP remove_assert_member members)
-End
-
-Definition compile_def:
-  compile dfy = from_program $ freshen_program $ remove_assert dfy
-End
-
-Definition env_rel_def:
-  env_rel env env' ⇔
-    env'.prog = remove_assert env.prog
-End
-
-Theorem env_rel_get_member_none_aux[local]:
-  get_member_aux name members = NONE ⇒
-  get_member_aux name (MAP remove_assert_member members) = NONE
-Proof
-  Induct_on ‘members’ >- (simp [])
-  \\ Cases \\ rpt strip_tac
-  \\ gvs [get_member_aux_def, remove_assert_member_def]
-QED
-
-Theorem env_rel_get_member_none[local]:
-  env_rel env env' ∧ get_member name env.prog = NONE ⇒
-  get_member name env'.prog = NONE
-Proof
-  rpt strip_tac
-  \\ gvs [env_rel_def]
-  \\ namedCases_on ‘env.prog’ ["members"]
-  \\ gvs [get_member_def, remove_assert_def]
-  \\ drule env_rel_get_member_none_aux \\ simp []
-QED
-
-Theorem env_rel_get_member_method_aux[local]:
-  get_member_aux name members =
-    SOME (Method name' ins req ens rds decrs outs mod body) ⇒
-  get_member_aux name (MAP remove_assert_member members) =
-    SOME
-      (Method name' ins req ens rds decrs outs mod (remove_assert_stmt body))
-Proof
-  Induct_on ‘members’ >- (simp [get_member_aux_def])
-  \\ Cases \\ rpt strip_tac
-  \\ gvs [get_member_aux_def, remove_assert_member_def]
-  \\ IF_CASES_TAC \\ gvs []
-QED
-
-Theorem env_rel_get_member_method[local]:
-  env_rel env env' ∧
-  get_member name env.prog =
-  SOME (Method name' ins req ens rds decrs outs mod body) ⇒
-  get_member name env'.prog =
-    SOME (Method name' ins req ens rds decrs outs mod (remove_assert_stmt body))
-Proof
-  rpt strip_tac
-  \\ gvs [env_rel_def]
-  \\ namedCases_on ‘env.prog’ ["members"]
-  \\ gvs [get_member_def, remove_assert_def]
-  \\ drule env_rel_get_member_method_aux \\ simp []
-QED
-
-Theorem env_rel_get_member_function_aux[local]:
-  get_member_aux name members =
-    SOME (Function name' ins res_t req rds decrs body) ⇒
-  get_member_aux name (MAP remove_assert_member members) =
-    SOME (Function name' ins res_t req rds decrs body)
-Proof
-  Induct_on ‘members’ >- (simp [])
-  \\ Cases \\ rpt strip_tac
-  \\ gvs [get_member_aux_def, remove_assert_member_def]
-  \\ IF_CASES_TAC \\ gvs []
-QED
-
-Theorem env_rel_get_member_function[local]:
-  env_rel env env' ∧
-  get_member name env.prog = r ∧
-  r = SOME (Function name' ins res_t req rds decrs body) ⇒
-  get_member name env'.prog = r
-Proof
-  rpt strip_tac
-  \\ gvs [env_rel_def]
-  \\ namedCases_on ‘env.prog’ ["members"]
-  \\ gvs [get_member_def, remove_assert_def]
-  \\ drule env_rel_get_member_function_aux \\ simp []
-QED
-
-Theorem env_rel_evaluate_exp[local]:
-  (∀s env' e env.
-     env_rel env env' ⇒ evaluate_exp s env' e = evaluate_exp s env e) ∧
-  (∀s env' es env.
-     env_rel env env' ⇒ evaluate_exps s env' es = evaluate_exps s env es)
-Proof
-  ho_match_mp_tac evaluate_exp_ind
-  \\ rpt strip_tac
-  >~ [‘Lit’] >- (gvs [evaluate_exp_def])
-  >~ [‘Var’] >- (gvs [evaluate_exp_def])
-  >~ [‘If’] >-
-   (gvs [evaluate_exp_def]
-    \\ last_x_assum $ drule_then assume_tac \\ simp []
-    \\ ntac 3 TOP_CASE_TAC \\ simp [])
-  >~ [‘UnOp’] >-
-   (gvs [evaluate_exp_def]
-    \\ last_x_assum $ drule_then assume_tac \\ simp [])
-  >~ [‘BinOp’] >-
-   (gvs [evaluate_exp_def]
-    \\ last_x_assum $ drule_then assume_tac \\ simp []
-    \\ ntac 3 TOP_CASE_TAC \\ gvs []
-    \\ last_x_assum $ drule_then assume_tac \\ simp [])
-  >~ [‘ArrLen’] >-
-   (gvs [evaluate_exp_def]
-    \\ last_x_assum $ drule_then assume_tac \\ simp [])
-  >~ [‘ArrSel’] >-
-   (gvs [evaluate_exp_def]
-    \\ last_x_assum $ drule_then assume_tac \\ simp []
-    \\ ntac 2 TOP_CASE_TAC \\ gvs []
-    \\ last_x_assum $ drule_then assume_tac \\ simp [])
-  >~ [‘FunCall’] >-
-   (gvs [evaluate_exp_def]
-    \\ namedCases_on ‘get_member name env.prog’ ["", "member"] \\ simp []
-    >- (drule_all_then assume_tac env_rel_get_member_none \\ simp [])
-    \\ Cases_on ‘member’ \\ simp []
-    >- (drule_all_then assume_tac env_rel_get_member_method \\ simp [])
-    >-
-     (drule env_rel_get_member_function \\ simp []
-      \\ disch_then $ drule_then assume_tac \\ gvs []
-      \\ first_x_assum $ drule_then assume_tac \\ simp []
-      \\ ntac 3 TOP_CASE_TAC
-      \\ IF_CASES_TAC \\ gvs []
-      \\ first_x_assum $ drule_then assume_tac \\ simp []))
-  >~ [‘Forall’] >-
-   (last_x_assum $ drule_then assume_tac
-    \\ gvs [evaluate_exp_def, eval_forall_def])
-  >~ [‘Old’] >-
-   (last_x_assum $ drule_then assume_tac \\ gvs [evaluate_exp_def])
-  >~ [‘OldHeap’] >-
-   (last_x_assum $ drule_then assume_tac \\ gvs [evaluate_exp_def])
-  >~ [‘Prev’] >-
-   (last_x_assum $ drule_then assume_tac \\ gvs [evaluate_exp_def])
-  >~ [‘PrevHeap’] >-
-   (last_x_assum $ drule_then assume_tac \\ gvs [evaluate_exp_def])
-  >~ [‘SetPrev’] >-
-   (last_x_assum $ drule_then assume_tac \\ gvs [evaluate_exp_def])
-  >~ [‘Let’] >-
-   (gvs [evaluate_exp_def]
-    \\ rpt (pairarg_tac \\ gvs [])
-    \\ IF_CASES_TAC \\ gvs []
-    \\ first_x_assum $ drule_then assume_tac \\ simp []
-    \\ ntac 2 TOP_CASE_TAC \\ gvs []
-    \\ first_x_assum $ drule_then assume_tac \\ simp [])
-  >~ [‘ForallHeap’] >-
-   (first_x_assum $ drule_then assume_tac
-    \\ gvs [evaluate_exp_def]
-    \\ ntac 3 TOP_CASE_TAC \\ gvs []
-    \\ first_x_assum $ drule_then assume_tac \\ simp [])
-  >~ [‘[]’] >- (gvs [evaluate_exp_def])
-  >~ [‘_::_’] >-
-   (first_x_assum $ drule_then assume_tac
-    \\ gvs [evaluate_exp_def]
-    \\ ntac 2 TOP_CASE_TAC \\ gvs []
-    \\ first_x_assum $ drule_then assume_tac \\ simp [])
-QED
-
-Theorem env_rel_evaluate_rhs_exp[local]:
-  env_rel env env' ⇒
-  evaluate_rhs_exp s env' e = evaluate_rhs_exp s env e
-Proof
-  strip_tac
-  \\ Cases_on ‘e’
-  >~ [‘ExpRhs’] >-
-   (simp [evaluate_rhs_exp_def]
-    \\ drule_then assume_tac (cj 1 env_rel_evaluate_exp) \\ simp [])
-  >~ [‘ArrAlloc’] >-
-   (simp [evaluate_rhs_exp_def]
-    \\ TOP_CASE_TAC
-    \\ drule_then assume_tac (cj 1 env_rel_evaluate_exp) \\ gvs [])
-QED
-
-Theorem env_rel_evaluate_rhs_exps[local]:
-  ∀s env' es env.
-    env_rel env env' ⇒
-    evaluate_rhs_exps s env' es = evaluate_rhs_exps s env es
-Proof
-  Induct_on ‘es’ >- (simp [evaluate_rhs_exps_def])
-  \\ rpt strip_tac
-  \\ simp [evaluate_rhs_exps_def]
-  \\ drule_then assume_tac env_rel_evaluate_rhs_exp \\ simp []
-  \\ ntac 2 TOP_CASE_TAC
-  \\ last_x_assum $ drule_then assume_tac \\ simp []
-QED
-
-Theorem env_rel_assign_value[local]:
-  env_rel env env' ⇒
-  assign_value s env' lhs rhs = assign_value s env lhs rhs
-Proof
-  strip_tac
-  \\ Cases_on ‘lhs’ >- (simp [assign_value_def])
-  \\ simp [assign_value_def]
-  \\ TOP_CASE_TAC
-  \\ drule_all_then assume_tac (cj 1 env_rel_evaluate_exp) \\ gvs []
-QED
-
-Theorem env_rel_assign_values[local]:
-  ∀s env' lhss rhss env.
-    env_rel env env' ⇒
-    assign_values s env' lhss rhss = assign_values s env lhss rhss
-Proof
-  ho_match_mp_tac assign_values_ind
-  \\ rpt strip_tac
-  \\ gvs [assign_values_def]
-  \\ drule_then assume_tac env_rel_assign_value \\ gvs []
-  \\ ntac 2 TOP_CASE_TAC \\ simp []
-QED
-
-Theorem correct_remove_assert_stmt:
-  ∀s env stmt s' env' r.
-    evaluate_stmt s env stmt = (s', r) ∧ env_rel env env' ∧
-    r ≠ Rstop (Serr Rfail) ∧ r ≠ Rstop (Serr Rtimeout) ⇒
-    evaluate_stmt s env' (remove_assert_stmt stmt) = (s', r)
-Proof
-  ho_match_mp_tac evaluate_stmt_ind
-  \\ simp [remove_assert_stmt_def]
-  \\ rpt strip_tac
-  >~ [‘Skip’] >- (gvs [evaluate_stmt_def])
-  >~ [‘Assert’] >-
-   (gvs [evaluate_stmt_def, AllCaseEqs()]
-    \\ rename [‘Rerr err’] \\ Cases_on ‘err’ \\ gvs [])
-  >~ [‘Then’] >- (gvs [evaluate_stmt_def, AllCaseEqs()])
-  >~ [‘If’] >-
-   (drule_then assume_tac (cj 1 env_rel_evaluate_exp)
-    \\ gvs [evaluate_stmt_def, oneline do_cond_def, AllCaseEqs()])
-  >~ [‘Dec local’] >-
-   (qpat_x_assum ‘evaluate_stmt _ _ _ = _ ’ mp_tac
-    \\ simp [evaluate_stmt_def]
-    \\ rpt (pairarg_tac \\ gvs [])
-    \\ TOP_CASE_TAC \\ rpt strip_tac \\ gvs [])
-  >~ [‘Assign’] >-
-   (gvs [evaluate_stmt_def]
-    \\ drule_then assume_tac env_rel_evaluate_rhs_exps \\ simp []
-    \\ ntac 2 TOP_CASE_TAC \\ gvs []
-    \\ drule_then assume_tac env_rel_assign_values \\ simp [])
-  >~ [‘While’] >-
-   (qpat_x_assum ‘evaluate_stmt _ _ _ = _’ mp_tac
-    \\ simp [evaluate_stmt_def]
-    \\ IF_CASES_TAC >- (simp [])
-    \\ simp []
-    \\ drule_then assume_tac (cj 1 env_rel_evaluate_exp) \\ simp []
-    \\ ntac 2 TOP_CASE_TAC
-    \\ IF_CASES_TAC >- (simp [])
-    \\ reverse IF_CASES_TAC >- (simp [])
-    \\ TOP_CASE_TAC
-    \\ reverse TOP_CASE_TAC >- (rpt strip_tac \\ gvs [])
-    \\ strip_tac \\ gvs []
-    \\ last_x_assum drule
-    \\ simp [STOP_def, remove_assert_stmt_def])
-  >~ [‘Print’] >-
-   (drule_then assume_tac (cj 1 env_rel_evaluate_exp)
-    \\ gvs [evaluate_stmt_def])
-  >~ [‘MetCall’] >-
-   (qpat_x_assum ‘evaluate_stmt _ _ _ = _’ mp_tac
-    \\ simp [evaluate_stmt_def]
-    \\ TOP_CASE_TAC >- (simp [])
-    \\ reverse TOP_CASE_TAC >- (simp [])
-    \\ drule_all_then assume_tac env_rel_get_member_method \\ simp []
-    \\ TOP_CASE_TAC
-    \\ drule_then assume_tac (cj 2 env_rel_evaluate_exp) \\ simp []
-    \\ ntac 2 TOP_CASE_TAC
-    \\ IF_CASES_TAC >- (simp [])
-    \\ simp []
-    \\ TOP_CASE_TAC
-    \\ TOP_CASE_TAC  >- (simp [])
-    \\ reverse TOP_CASE_TAC >- (rpt strip_tac \\ gvs [])
-    \\ gvs []
-    \\ TOP_CASE_TAC
-    \\ IF_CASES_TAC >- (simp [])
-    \\ simp []
-    \\ strip_tac \\ drule env_rel_assign_values \\ simp [])
-  >~ [‘Return’] >- (gvs [evaluate_stmt_def])
-QED
-
-Theorem member_name_remove_assert_member_eq[local]:
-  MAP member_name (MAP remove_assert_member members) =
-  MAP member_name members
-Proof
-  Induct_on ‘members’ >- (simp [])
-  \\ Cases \\ gvs [remove_assert_member_def]
-QED
-
-Theorem correct_remove_assert:
-  evaluate_program ck prog = (s,Rcont) ⇒
-  evaluate_program ck (remove_assert prog) = (s,Rcont)
-Proof
-  namedCases_on ‘prog’ ["members"]
-  \\ simp [remove_assert_def, evaluate_program_def]
-  \\ simp [member_name_remove_assert_member_eq]
-  \\ IF_CASES_TAC \\ simp []
-  \\ simp [mk_env_def]
-  \\ strip_tac
-  \\ drule correct_remove_assert_stmt \\ simp [remove_assert_stmt_def]
-  \\ disch_then irule
-  \\ simp [env_rel_def, remove_assert_def]
-QED
-
-Theorem has_main_remove_assert[local]:
-  has_main (remove_assert prog) = has_main prog
-Proof
-  namedCases_on ‘prog’ ["members"]
-  \\ simp [remove_assert_def]
-  \\ Induct_on ‘members’
-  >- (simp [remove_assert_member_def])
-  \\ qx_gen_tac ‘member’
-  \\ gvs [has_main_def, get_member_def, get_member_aux_def]
-  \\ Cases_on ‘member’ \\ simp [remove_assert_member_def]
-  \\ IF_CASES_TAC \\ gvs []
-QED
-
-Theorem valid_members_remove_assert[local]:
-  valid_members prog ⇒ valid_members (remove_assert prog)
-Proof
-  namedCases_on ‘prog’ ["members"]
-  \\ simp [valid_members_def, remove_assert_def]
-  \\ Induct_on ‘members’ >- (simp [])
-  \\ Cases \\ rpt strip_tac \\ gvs []
-  \\ simp [remove_assert_member_def, get_param_names_def]
-QED
+(* Establish no_assert from remove_assert and preserve it throughout the
+   compiler passes*)
 
 Definition no_assert_def:
   no_assert (Program members) = EVERY no_assert_member members
@@ -501,6 +169,10 @@ Proof
   \\ rpt strip_tac \\ fs []
   \\ drule no_assert_member_freshen_member \\ simp []
 QED
+
+(* -- *)
+
+(* Top-level compiler correctness result *)
 
 Theorem correct_compile:
   ∀dfy_ck prog s cml_decs (ffi: 'ffi ffi_state).
