compiler/dafny/proofs/dafny_remove_assertProofScript.sml
@@ -1,0 +1,303 @@
+(*
+  Show that removing assert preserves semantics of "good" programs.
+*)
+Theory dafny_remove_assertProof
+Ancestors
+  dafny_semanticPrimitives
+  dafny_evaluate
+  dafny_remove_assert
+Libs
+  preamble
+
+Definition env_rel_def:
+  env_rel env env' ⇔
+    env'.prog = remove_assert env.prog
+End
+
+Theorem env_rel_get_member_none_aux[local]:
+  get_member_aux name members = NONE ⇒
+  get_member_aux name (MAP remove_assert_member members) = NONE
+Proof
+  Induct_on ‘members’ >- (simp [])
+  \\ Cases \\ rpt strip_tac
+  \\ gvs [get_member_aux_def, remove_assert_member_def]
+QED
+
+Theorem env_rel_get_member_none[local]:
+  env_rel env env' ∧ get_member name env.prog = NONE ⇒
+  get_member name env'.prog = NONE
+Proof
+  rpt strip_tac
+  \\ gvs [env_rel_def]
+  \\ namedCases_on ‘env.prog’ ["members"]
+  \\ gvs [get_member_def, remove_assert_def]
+  \\ drule env_rel_get_member_none_aux \\ simp []
+QED
+
+Theorem env_rel_get_member_method_aux[local]:
+  get_member_aux name members =
+    SOME (Method name' ins req ens rds decrs outs mod body) ⇒
+  get_member_aux name (MAP remove_assert_member members) =
+    SOME
+      (Method name' ins req ens rds decrs outs mod (remove_assert_stmt body))
+Proof
+  Induct_on ‘members’ >- (simp [get_member_aux_def])
+  \\ Cases \\ rpt strip_tac
+  \\ gvs [get_member_aux_def, remove_assert_member_def]
+  \\ IF_CASES_TAC \\ gvs []
+QED
+
+Theorem env_rel_get_member_method[local]:
+  env_rel env env' ∧
+  get_member name env.prog =
+  SOME (Method name' ins req ens rds decrs outs mod body) ⇒
+  get_member name env'.prog =
+    SOME (Method name' ins req ens rds decrs outs mod (remove_assert_stmt body))
+Proof
+  rpt strip_tac
+  \\ gvs [env_rel_def]
+  \\ namedCases_on ‘env.prog’ ["members"]
+  \\ gvs [get_member_def, remove_assert_def]
+  \\ drule env_rel_get_member_method_aux \\ simp []
+QED
+
+Theorem env_rel_get_member_function_aux[local]:
+  get_member_aux name members =
+    SOME (Function name' ins res_t req rds decrs body) ⇒
+  get_member_aux name (MAP remove_assert_member members) =
+    SOME (Function name' ins res_t req rds decrs body)
+Proof
+  Induct_on ‘members’ >- (simp [])
+  \\ Cases \\ rpt strip_tac
+  \\ gvs [get_member_aux_def, remove_assert_member_def]
+  \\ IF_CASES_TAC \\ gvs []
+QED
+
+Theorem env_rel_get_member_function[local]:
+  env_rel env env' ∧
+  get_member name env.prog = r ∧
+  r = SOME (Function name' ins res_t req rds decrs body) ⇒
+  get_member name env'.prog = r
+Proof
+  rpt strip_tac
+  \\ gvs [env_rel_def]
+  \\ namedCases_on ‘env.prog’ ["members"]
+  \\ gvs [get_member_def, remove_assert_def]
+  \\ drule env_rel_get_member_function_aux \\ simp []
+QED
+
+Theorem env_rel_evaluate_exp[local]:
+  (∀s env' e env.
+     env_rel env env' ⇒ evaluate_exp s env' e = evaluate_exp s env e) ∧
+  (∀s env' es env.
+     env_rel env env' ⇒ evaluate_exps s env' es = evaluate_exps s env es)
+Proof
+  ho_match_mp_tac evaluate_exp_ind
+  \\ rpt strip_tac
+  >~ [‘Lit’] >- (gvs [evaluate_exp_def])
+  >~ [‘Var’] >- (gvs [evaluate_exp_def])
+  >~ [‘If’] >-
+   (gvs [evaluate_exp_def]
+    \\ last_x_assum $ drule_then assume_tac \\ simp []
+    \\ ntac 3 TOP_CASE_TAC \\ simp [])
+  >~ [‘UnOp’] >-
+   (gvs [evaluate_exp_def]
+    \\ last_x_assum $ drule_then assume_tac \\ simp [])
+  >~ [‘BinOp’] >-
+   (gvs [evaluate_exp_def]
+    \\ last_x_assum $ drule_then assume_tac \\ simp []
+    \\ ntac 3 TOP_CASE_TAC \\ gvs []
+    \\ last_x_assum $ drule_then assume_tac \\ simp [])
+  >~ [‘ArrLen’] >-
+   (gvs [evaluate_exp_def]
+    \\ last_x_assum $ drule_then assume_tac \\ simp [])
+  >~ [‘ArrSel’] >-
+   (gvs [evaluate_exp_def]
+    \\ last_x_assum $ drule_then assume_tac \\ simp []
+    \\ ntac 2 TOP_CASE_TAC \\ gvs []
+    \\ last_x_assum $ drule_then assume_tac \\ simp [])
+  >~ [‘FunCall’] >-
+   (gvs [evaluate_exp_def]
+    \\ namedCases_on ‘get_member name env.prog’ ["", "member"] \\ simp []
+    >- (drule_all_then assume_tac env_rel_get_member_none \\ simp [])
+    \\ Cases_on ‘member’ \\ simp []
+    >- (drule_all_then assume_tac env_rel_get_member_method \\ simp [])
+    >-
+     (drule env_rel_get_member_function \\ simp []
+      \\ disch_then $ drule_then assume_tac \\ gvs []
+      \\ first_x_assum $ drule_then assume_tac \\ simp []
+      \\ ntac 3 TOP_CASE_TAC
+      \\ IF_CASES_TAC \\ gvs []
+      \\ first_x_assum $ drule_then assume_tac \\ simp []))
+  >~ [‘Forall’] >-
+   (last_x_assum $ drule_then assume_tac
+    \\ gvs [evaluate_exp_def, eval_forall_def])
+  >~ [‘Old’] >-
+   (last_x_assum $ drule_then assume_tac \\ gvs [evaluate_exp_def])
+  >~ [‘OldHeap’] >-
+   (last_x_assum $ drule_then assume_tac \\ gvs [evaluate_exp_def])
+  >~ [‘Prev’] >-
+   (last_x_assum $ drule_then assume_tac \\ gvs [evaluate_exp_def])
+  >~ [‘PrevHeap’] >-
+   (last_x_assum $ drule_then assume_tac \\ gvs [evaluate_exp_def])
+  >~ [‘SetPrev’] >-
+   (last_x_assum $ drule_then assume_tac \\ gvs [evaluate_exp_def])
+  >~ [‘Let’] >-
+   (gvs [evaluate_exp_def]
+    \\ rpt (pairarg_tac \\ gvs [])
+    \\ IF_CASES_TAC \\ gvs []
+    \\ first_x_assum $ drule_then assume_tac \\ simp []
+    \\ ntac 2 TOP_CASE_TAC \\ gvs []
+    \\ first_x_assum $ drule_then assume_tac \\ simp [])
+  >~ [‘ForallHeap’] >-
+   (first_x_assum $ drule_then assume_tac
+    \\ gvs [evaluate_exp_def]
+    \\ ntac 3 TOP_CASE_TAC \\ gvs []
+    \\ first_x_assum $ drule_then assume_tac \\ simp [])
+  >~ [‘[]’] >- (gvs [evaluate_exp_def])
+  >~ [‘_::_’] >-
+   (first_x_assum $ drule_then assume_tac
+    \\ gvs [evaluate_exp_def]
+    \\ ntac 2 TOP_CASE_TAC \\ gvs []
+    \\ first_x_assum $ drule_then assume_tac \\ simp [])
+QED
+
+Theorem env_rel_evaluate_rhs_exp[local]:
+  env_rel env env' ⇒
+  evaluate_rhs_exp s env' e = evaluate_rhs_exp s env e
+Proof
+  strip_tac
+  \\ Cases_on ‘e’
+  >~ [‘ExpRhs’] >-
+   (simp [evaluate_rhs_exp_def]
+    \\ drule_then assume_tac (cj 1 env_rel_evaluate_exp) \\ simp [])
+  >~ [‘ArrAlloc’] >-
+   (simp [evaluate_rhs_exp_def]
+    \\ TOP_CASE_TAC
+    \\ drule_then assume_tac (cj 1 env_rel_evaluate_exp) \\ gvs [])
+QED
+
+Theorem env_rel_evaluate_rhs_exps[local]:
+  ∀s env' es env.
+    env_rel env env' ⇒
+    evaluate_rhs_exps s env' es = evaluate_rhs_exps s env es
+Proof
+  Induct_on ‘es’ >- (simp [evaluate_rhs_exps_def])
+  \\ rpt strip_tac
+  \\ simp [evaluate_rhs_exps_def]
+  \\ drule_then assume_tac env_rel_evaluate_rhs_exp \\ simp []
+  \\ ntac 2 TOP_CASE_TAC
+  \\ last_x_assum $ drule_then assume_tac \\ simp []
+QED
+
+Theorem env_rel_assign_value[local]:
+  env_rel env env' ⇒
+  assign_value s env' lhs rhs = assign_value s env lhs rhs
+Proof
+  strip_tac
+  \\ Cases_on ‘lhs’ >- (simp [assign_value_def])
+  \\ simp [assign_value_def]
+  \\ TOP_CASE_TAC
+  \\ drule_all_then assume_tac (cj 1 env_rel_evaluate_exp) \\ gvs []
+QED
+
+Theorem env_rel_assign_values[local]:
+  ∀s env' lhss rhss env.
+    env_rel env env' ⇒
+    assign_values s env' lhss rhss = assign_values s env lhss rhss
+Proof
+  ho_match_mp_tac assign_values_ind
+  \\ rpt strip_tac
+  \\ gvs [assign_values_def]
+  \\ drule_then assume_tac env_rel_assign_value \\ gvs []
+  \\ ntac 2 TOP_CASE_TAC \\ simp []
+QED
+
+Theorem correct_remove_assert_stmt:
+  ∀s env stmt s' env' r.
+    evaluate_stmt s env stmt = (s', r) ∧ env_rel env env' ∧
+    r ≠ Rstop (Serr Rfail) ∧ r ≠ Rstop (Serr Rtimeout) ⇒
+    evaluate_stmt s env' (remove_assert_stmt stmt) = (s', r)
+Proof
+  ho_match_mp_tac evaluate_stmt_ind
+  \\ simp [remove_assert_stmt_def]
+  \\ rpt strip_tac
+  >~ [‘Skip’] >- (gvs [evaluate_stmt_def])
+  >~ [‘Assert’] >-
+   (gvs [evaluate_stmt_def, AllCaseEqs()]
+    \\ rename [‘Rerr err’] \\ Cases_on ‘err’ \\ gvs [])
+  >~ [‘Then’] >- (gvs [evaluate_stmt_def, AllCaseEqs()])
+  >~ [‘If’] >-
+   (drule_then assume_tac (cj 1 env_rel_evaluate_exp)
+    \\ gvs [evaluate_stmt_def, oneline do_cond_def, AllCaseEqs()])
+  >~ [‘Dec local’] >-
+   (qpat_x_assum ‘evaluate_stmt _ _ _ = _ ’ mp_tac
+    \\ simp [evaluate_stmt_def]
+    \\ rpt (pairarg_tac \\ gvs [])
+    \\ TOP_CASE_TAC \\ rpt strip_tac \\ gvs [])
+  >~ [‘Assign’] >-
+   (gvs [evaluate_stmt_def]
+    \\ drule_then assume_tac env_rel_evaluate_rhs_exps \\ simp []
+    \\ ntac 2 TOP_CASE_TAC \\ gvs []
+    \\ drule_then assume_tac env_rel_assign_values \\ simp [])
+  >~ [‘While’] >-
+   (qpat_x_assum ‘evaluate_stmt _ _ _ = _’ mp_tac
+    \\ simp [evaluate_stmt_def]
+    \\ IF_CASES_TAC >- (simp [])
+    \\ simp []
+    \\ drule_then assume_tac (cj 1 env_rel_evaluate_exp) \\ simp []
+    \\ ntac 2 TOP_CASE_TAC
+    \\ IF_CASES_TAC >- (simp [])
+    \\ reverse IF_CASES_TAC >- (simp [])
+    \\ TOP_CASE_TAC
+    \\ reverse TOP_CASE_TAC >- (rpt strip_tac \\ gvs [])
+    \\ strip_tac \\ gvs []
+    \\ last_x_assum drule
+    \\ simp [STOP_def, remove_assert_stmt_def])
+  >~ [‘Print’] >-
+   (drule_then assume_tac (cj 1 env_rel_evaluate_exp)
+    \\ gvs [evaluate_stmt_def])
+  >~ [‘MetCall’] >-
+   (qpat_x_assum ‘evaluate_stmt _ _ _ = _’ mp_tac
+    \\ simp [evaluate_stmt_def]
+    \\ TOP_CASE_TAC >- (simp [])
+    \\ reverse TOP_CASE_TAC >- (simp [])
+    \\ drule_all_then assume_tac env_rel_get_member_method \\ simp []
+    \\ TOP_CASE_TAC
+    \\ drule_then assume_tac (cj 2 env_rel_evaluate_exp) \\ simp []
+    \\ ntac 2 TOP_CASE_TAC
+    \\ IF_CASES_TAC >- (simp [])
+    \\ simp []
+    \\ TOP_CASE_TAC
+    \\ TOP_CASE_TAC  >- (simp [])
+    \\ reverse TOP_CASE_TAC >- (rpt strip_tac \\ gvs [])
+    \\ gvs []
+    \\ TOP_CASE_TAC
+    \\ IF_CASES_TAC >- (simp [])
+    \\ simp []
+    \\ strip_tac \\ drule env_rel_assign_values \\ simp [])
+  >~ [‘Return’] >- (gvs [evaluate_stmt_def])
+QED
+
+Theorem member_name_remove_assert_member_eq[local]:
+  MAP member_name (MAP remove_assert_member members) =
+  MAP member_name members
+Proof
+  Induct_on ‘members’ >- (simp [])
+  \\ Cases \\ gvs [remove_assert_member_def]
+QED
+
+Theorem correct_remove_assert:
+  evaluate_program ck prog = (s,Rcont) ⇒
+  evaluate_program ck (remove_assert prog) = (s,Rcont)
+Proof
+  namedCases_on ‘prog’ ["members"]
+  \\ simp [remove_assert_def, evaluate_program_def]
+  \\ simp [member_name_remove_assert_member_eq]
+  \\ IF_CASES_TAC \\ simp []
+  \\ simp [mk_env_def]
+  \\ strip_tac
+  \\ drule correct_remove_assert_stmt \\ simp [remove_assert_stmt_def]
+  \\ disch_then irule
+  \\ simp [env_rel_def, remove_assert_def]
+QED
